Generalized PutBot into PutLab

ifc/extended/Machine/Instructions.v
@@ -15,28 +15,32 @@ Definition eval_binop (b : BinOpT) : Z -> Z -> option Z :=
     | BMult => fun z1 z2 => Some (z1 * z2)%Z
   end.
 
-Inductive Instruction : Type :=
-  | Lab      : regId -> regId -> Instruction
-  | MLab     : regId -> regId -> Instruction
-  | PcLab    : regId -> Instruction
-  | BCall    : regId -> regId -> regId -> Instruction
-  | BRet     : Instruction
-  | FlowsTo  : regId -> regId -> regId -> Instruction
-  | LJoin    : regId -> regId -> regId -> Instruction
-  | PutBot   : regId -> Instruction
-  | Nop      : Instruction
-  | Put (n : Z) : regId -> Instruction
-  | BinOp (o : BinOpT) : regId -> regId -> regId -> Instruction
-  | Jump     : regId -> Instruction
-  | BNZ (n : Z) : regId -> Instruction
-  | Load     : regId -> regId -> Instruction
-  | Store    : regId -> regId -> Instruction
-  | Alloc    : regId -> regId -> regId -> Instruction
-  | PSetOff  : regId -> regId -> regId -> Instruction
-  | Output   : regId -> Instruction
-  | Halt     : Instruction
-  | PGetOff  : regId -> regId -> Instruction
-  | MSize    : regId -> regId -> Instruction.
+Section Instr.
+
+Context {Label : Type}.
+
+Inductive Instr : Type :=
+  | Lab      : regId -> regId -> Instr
+  | MLab     : regId -> regId -> Instr
+  | PcLab    : regId -> Instr
+  | BCall    : regId -> regId -> regId -> Instr
+  | BRet     : Instr
+  | FlowsTo  : regId -> regId -> regId -> Instr
+  | LJoin    : regId -> regId -> regId -> Instr
+  | PutLab   : Label -> regId -> Instr
+  | Nop      : Instr
+  | Put (n : Z) : regId -> Instr
+  | BinOp (o : BinOpT) : regId -> regId -> regId -> Instr
+  | Jump     : regId -> Instr
+  | BNZ (n : Z) : regId -> Instr
+  | Load     : regId -> regId -> Instr
+  | Store    : regId -> regId -> Instr
+  | Alloc    : regId -> regId -> regId -> Instr
+  | PSetOff  : regId -> regId -> regId -> Instr
+  | Output   : regId -> Instr
+  | Halt     : Instr
+  | PGetOff  : regId -> regId -> Instr
+  | MSize    : regId -> regId -> Instr.
 
 Inductive OpCode : Type :=
   | OpLab
@@ -46,7 +50,7 @@ Inductive OpCode : Type :=
   | OpBRet
   | OpFlowsTo
   | OpLJoin
-  | OpPutBot
+  | OpPutLab
   | OpNop
   | OpPut
   | OpBinOp
@@ -68,7 +72,7 @@ Definition opCodes :=
   ; OpBRet
   ; OpFlowsTo
   ; OpLJoin
-  ; OpPutBot
+  ; OpPutLab
   ; OpNop
   ; OpPut
   ; OpBinOp
@@ -89,7 +93,7 @@ Definition opCode_eq_dec : forall o1 o2 : OpCode,
   {o1 = o2} + {o1 <> o2}.
 Proof. decide equality. Defined.
 
-Definition opcode_of_instr (i : Instruction) : option OpCode :=
+Definition opcode_of_instr (i : Instr) : option OpCode :=
   match i with
   | Lab _ _       => Some OpLab
   | MLab _ _      => Some OpMLab
@@ -98,7 +102,7 @@ Definition opcode_of_instr (i : Instruction) : option OpCode :=
   | BRet          => Some OpBRet
   | FlowsTo _ _ _ => Some OpFlowsTo
   | LJoin _ _ _   => Some OpLJoin
-  | PutBot _      => Some OpPutBot
+  | PutLab _ _    => Some OpPutLab
   | Nop           => Some OpNop
   | Put _ _       => Some OpPut
   | BinOp _ _ _ _ => Some OpBinOp
@@ -111,5 +115,7 @@ Definition opcode_of_instr (i : Instruction) : option OpCode :=
   | Output _      => Some OpOutput
   | PGetOff _ _   => Some OpPGetOff
   | MSize _ _     => Some OpMSize
-  | _             => None (* CH: halt has no opcode? why? *)
+  | Halt          => None (* CH: halt has no opcode? why? *)
 end.
+
+End Instr.
